format-version: 1.2
date: 25:02:2021 10:56
saved-by: pfey
auto-generated-by: OBO-Edit 2.2
default-namespace: Dicty Developmental Stages

[Term]
id: DDDEV:0000001
name: developmental stage
def: "Any developmental stage during Dictyostelium discoideum development." [DDB:pf]
creation_date: 2021-02-01T10:13:52Z

[Term]
id: DDDEV:0000002
name: mound stage
def: "Post aggregative cells forming a mound during Dictyostelium development." [DDB:pf]
synonym: "aggregate stage" EXACT []
synonym: "tight mound stage" NARROW []
is_a: DDDEV:0000001 ! developmental stage
created_by: pfey
creation_date: 2021-02-01T10:16:33Z

[Term]
id: DDDEV:0000003
name: loose mound stage
def: "Adherent cell mass early during Dictyostelium development." [DDB:pf]
synonym: "loose aggregate stage" EXACT []
is_a: DDDEV:0000002 ! mound stage
created_by: pfey
creation_date: 2021-02-01T10:19:48Z

[Term]
id: DDDEV:0000004
name: tipped mound stage
def: "Aggregated cells that undergo development and form a tip." [DDB:pf]
synonym: "tipped aggregate stage" EXACT []
is_a: DDDEV:0000002 ! mound stage
created_by: pfey
creation_date: 2021-02-01T10:53:59Z

[Term]
id: DDDEV:0000005
name: standing slug stage
def: "Structure formed by elongation of the mound under the control of the tip." [DDB:pf]
synonym: "finger stage" EXACT []
is_a: DDDEV:0000006 ! slug stage
created_by: pfey
creation_date: 2021-02-01T10:57:03Z

[Term]
id: DDDEV:0000006
name: slug stage
def: "In sub-optimal conditions for development, the standing slug bends over and migrates towards more favorable environmental conditions." [DDB:pf]
synonym: "migratory slug stage" EXACT []
is_a: DDDEV:0000001 ! developmental stage
created_by: pfey
creation_date: 2021-02-01T11:00:23Z

[Term]
id: DDDEV:0000007
name: early culminant stage
def: "Structure after standing slug or slug migration when the cell mass moves under the tip, when the stalk tube starts forming." [DDB:pf]
synonym: "mexican hat stage" NARROW []
is_a: DDDEV:0000001 ! developmental stage
created_by: pfey
creation_date: 2021-02-01T11:13:28Z

[Term]
id: DDDEV:0000008
name: mid culminant stage
def: "Structure in which stalk tube formation has progressed and lifts the prespore mass off the ground." [DDB:pf]
synonym: "culminant stage" BROAD []
is_a: DDDEV:0000001 ! developmental stage
created_by: pfey
creation_date: 2021-02-01T11:19:54Z

[Term]
id: DDDEV:0000009
name: late culminant stage
def: "Structure in which stalk tube formation has progressed and the sorogen ascends, stalk vacuolization and spore differentiation begins." [DDB:pf]
synonym: "culminant stage" BROAD []
is_a: DDDEV:0000001 ! developmental stage
created_by: pfey
creation_date: 2021-02-01T11:23:33Z

[Term]
id: DDDEV:0000010
name: fruiting body
def: "End of asexual development,  terminally differentiated consisting of a long stalk on top of which sits the sorus containing spores, measuring 1.5-3 mm in height." [DDB:pf]
synonym: "sorocarp" EXACT []
is_a: DDDEV:0000001 ! developmental stage
created_by: pfey
creation_date: 2021-02-01T11:28:10Z

